휴, lemma_to_seq 증명 성공!

src/regular/Nemonuri.AbstractSet.BitVector.fst
@@ -5,6 +5,7 @@ module USet = Nemonuri.AbstractSet.Under
 module S = FStar.Seq
 module Ss = FStar.Seq.Sorted
 module Sto = Nemonuri.StrictTotalOrder
+module I = FStar.IntegerIntervals
 
 type t (capacity: nat) : eqtype = Bv.bv_t capacity
 
@@ -19,7 +20,9 @@ let is_greater (a b:int) : prop = a < b
 let lemma_is_greater () : Lemma (Sto.is_well_defined is_greater) = ()
 
 private let rec to_seq_core' #c (set: t c) (index: USet.t (c+1))
-  : Tot (S.seq (USet.t c)) 
+  : Pure (S.seq (USet.t c)) 
+         (requires True)
+         (ensures (fun r -> S.for_all ((<=) index) r))
          (decreases (S.length set) - index)
   =
   if index = c then S.empty
@@ -50,70 +53,34 @@ let lemma_to_seq_length #c (set: t c)
   in
   prove_induct_decr 0 (c+1) pred lemma_step' (assert (S.length (to_seq_core' set c) == 0))
 
-(*
 let lemma_to_seq #c (set: t c) 
   : Lemma (Sto.is_sorted is_greater (to_seq set)) =
-  assert (S.length == c);
-  let sorted' = (Sto.is_sorted is_greater) in
+  assert (S.length set == c);
+  let open Nemonuri.Squash in
   if (c = 0) then () 
-  else if (c = 1) then Sto.lemma_singleton binrel 
-  else begin
-    let lemma_aux' #c (set: t c) (index: USet.t c)
-      : Lemma (requires sorted' (to_seq_core' set c index)) 
-              (ensures  )
+  else if (c = 1) then begin
+    let to_seq_length = S.length (to_seq set) in
+    prove (to_seq_length <= 1) (lemma_to_seq_length set);
+    match to_seq_length with
+    | 0 -> ()
+    | 1 -> Sto.lemma_singleton_seq is_greater (to_seq set) 
+  end else begin
+    assert (c >= 2);
+    let step_pred (index:USet.t (c+1)) : prop = Sto.is_sorted is_greater (to_seq_core' set index) in
+    let lemma_aux' (index: USet.t (c+1){index > 0})
+      : Lemma (requires step_pred index) 
+              (ensures step_pred (index-1))
       =
-
+      let p_goal = step_pred (index-1) in
+      let index' = index-1 in
+      let tail_seq = to_seq_core' set (index'+1) in
+      let cons_seq = S.cons index' tail_seq in
+      if contains set index' then begin 
+        assert (Sto.compare_head is_greater index' tail_seq);
+        Sto.lemma_cons is_greater index' tail_seq;
+        assert p_goal
+      end else assert p_goal
     in
+    prove_induct_decr 0 (c+1) step_pred lemma_aux' (assert (S.length (to_seq_core' set c) == 0))
   end
-*)
-
-//private let rec lemma_to_set_core' #c (set: t c) (index: USet.t (c+1))
-//  : Lemma (ensures Sto.is_sorted is_greater (to_set_core' set index))
-//          (decreases (S.length set) - index)
-//  =
-
-
-(*
-private let to_seq_core' #c (set: t c) (index: USet.t (c+1)) (prev_result: S.seq (USet.t c))
-  : Pure (S.seq (USet.t c)) 
-      (requires (S.sorted (<=) prev_result) /\ ((S.length prev_result > 0) ==> (index <= S.head prev_result)))
-      (ensures (fun r -> S.sorted (<=) r))
-  =
-  if index = c then S.empty
-  else 
-    //let tail_part = (to_seq_core' set (index+1)) in
-    if contains set index then begin
-      let result = S.cons index prev_result in
-      if S.length result > 1 
-      then begin
-        S.cons_head_tail result;
-        assume (prev_result == (S.tail result));
-        assert (S.sorted (<=) (S.tail result));
-        Ss.sorted_pred_cons_lemma (<=) result
-      end else ();
-      result
-    end else prev_result
-*)
-
-(*
-private let rec lemma_to_seq_core' #c (set: t c) (index: USet.t (c+1))
-  : Lemma (ensures S.sorted (<=) (to_seq_core' set index)) (decreases (S.length set) - index) =
-  if index = c then ()
-  else 
-    let tail_part = (to_seq_core' set (index+1)) in
-    if contains set index 
-    then if S.length tail_part = 0 then () else 
-      begin
-        assert (index < (S.head tail_part));
-        lemma_to_seq_core' #c set (index+1)
-      end
-    else lemma_to_seq_core' #c set (index+1)
-*)
-
-
-  
-
-
-
-
 
